copy_exact, copy_strong

src/lowparse/LowParse.SteelSel.Access.fst
@@ -24,7 +24,7 @@ let parsed_size
       U32.v res == A.length (h (vparse p a)).array
     )
 
-let parsed_size_total_constant_size' // OK, but mostly not used
+let parsed_size_total_constant_size
   (#k: parser_kind)
   (#t: Type)
   (p: parser k t)
@@ -103,4 +103,112 @@ let peek_strong
   parse_strong_prefix p c_a.AP.contents (Seq.slice c_a.AP.contents 0 (U32.v n)); 
   let res = AP.split a n in
   intro_vparse p a;
+  SEA.return res
+
+(* TODO: move to Steel.SelArray *)
+val memcpy
+  (dst: byte_array)
+  (src: byte_array)
+  (n: U32.t)
+: SE.SteelSel byte_array
+    (AP.varrayptr dst `SE.star` AP.varrayptr src)
+    (fun _ -> AP.varrayptr dst `SE.star` AP.varrayptr src)
+    (fun h ->
+      U32.v n <= A.length (h (AP.varrayptr src)).AP.array /\
+      U32.v n <= A.length (h (AP.varrayptr dst)).AP.array
+    )
+    (fun h res h' ->
+      let s = h (AP.varrayptr src) in
+      let d = h (AP.varrayptr dst) in
+      let d' = h' (AP.varrayptr dst) in
+      res == dst /\
+      h' (AP.varrayptr src) == s /\
+      d'.AP.array == d.AP.array /\
+      U32.v n <= A.length d.AP.array /\
+      U32.v n <= A.length s.AP.array /\
+      d'.AP.contents `Seq.equal` (Seq.slice s.AP.contents 0 (U32.v n) `Seq.append` Seq.slice d.AP.contents (U32.v n) (A.length d.AP.array))
+    )
+    (decreases (U32.v n))
+
+let rec memcpy dst src n =
+  if n = 0ul
+  then SEA.return dst
+  else begin
+    let j = n `U32.sub` 1ul in
+    let c = AP.index src j in
+    AP.upd dst j c;
+    memcpy dst src j
+  end
+
+val copy_exact
+  (#k: parser_kind)
+  (#t: Type)
+  (p: parser k t)
+  (src: byte_array)
+  (dst: byte_array)
+  (n: U32.t)
+: SE.SteelSel unit
+    (vparse p src `SE.star` AP.varrayptr dst)
+    (fun _ -> vparse p src `SE.star` vparse p dst)
+    (fun h ->
+      U32.v n == A.length (h (vparse p src)).array /\
+      U32.v n == A.length (h (AP.varrayptr dst)).AP.array
+    )
+    (fun h _ h' ->
+      let s = h (vparse p src) in
+      let d = h (AP.varrayptr dst) in
+      let d' = h' (vparse p dst) in
+      U32.v n == A.length s.array /\
+      U32.v n == A.length d.AP.array /\
+      h' (vparse p src) == s /\
+      d'.array == d.AP.array /\
+      d'.contents == s.contents
+    )
+
+let copy_exact p src dst n =
+  elim_vparse p src;
+  let _ = memcpy dst src n in
+  let gs : Ghost.erased (AP.v byte) = SEA.gget (AP.varrayptr src) in
+  assert (U32.v n == A.length gs.AP.array); // FIXME: WHY WHY WHY is this needed for the equality on n in the postcond
+  let gd : Ghost.erased (AP.v byte) = SEA.gget (AP.varrayptr dst) in
+  assert (U32.v n == A.length gd.AP.array); // same here
+  assert (gd.AP.contents `Seq.equal` gs.AP.contents); // ok, this is expected because of `equal`
+  intro_vparse p src;
+  intro_vparse p dst
+
+val copy_strong
+  (#k: parser_kind)
+  (#t: Type)
+  (#p: parser k t)
+  (j: parsed_size p)
+  (src: byte_array)
+  (dst: byte_array)
+: SE.SteelSel byte_array
+    (vparse p src `SE.star` AP.varrayptr dst)
+    (fun res -> vparse p src `SE.star` vparse p dst `SE.star` AP.varrayptr res)
+    (fun h ->
+      A.length (h (vparse p src)).array <= A.length (h (AP.varrayptr dst)).AP.array
+    )
+    (fun h res h' ->
+      SE.can_be_split (vparse p src `SE.star` vparse p dst `SE.star` AP.varrayptr res) (vparse p src) /\ // FIXME: WHY WHY WHY?
+      SE.can_be_split (vparse p src `SE.star` vparse p dst `SE.star` AP.varrayptr res) (vparse p dst) /\ // same here
+      begin
+        let s = h (vparse p src) in
+        let d = h (AP.varrayptr dst) in
+        let d' = h' (vparse p dst) in
+        let r = h' (AP.varrayptr res) in
+        h' (vparse p src) == s /\
+        A.merge_into d'.array r.AP.array d.AP.array /\
+        d'.contents == s.contents /\
+        A.length s.array == A.length d'.array /\ // TODO: this should be a consequence of the equality of the contents, via parser injectivity
+        r.AP.contents == Seq.slice d.AP.contents (A.length s.array) (A.length d.AP.array)
+      end
+    )
+
+let copy_strong #_ #_ #p j src dst =
+  let n = j src in
+  let res = AP.split dst n in
+  let _ = SEA.gget (AP.varrayptr dst) in // FIXME: WHY WHY WHY?
+  copy_exact p src dst n;
+  SEA.reveal_star_3 (vparse p src) (vparse p dst) (AP.varrayptr res); // for can_be_split
   SEA.return res
